tuned
--HG--
extra : rebase_source : d7ba310400cd8f63ff2a4c96004abd123401ddf0

src/HOL/Library/Comparator.thy
@@ -13,146 +13,146 @@ subsection \<open>Basic properties\<close>
 datatype comp = Less | Equiv | Greater
 
 locale comparator =
-  fixes cmp :: "'a \<Rightarrow> 'a \<Rightarrow> comp"
-  assumes refl [simp]: "\<And>a. cmp a a = Equiv"
-    and trans_equiv: "\<And>a b c. cmp a b = Equiv \<Longrightarrow> cmp b c = Equiv \<Longrightarrow> cmp a c = Equiv"
-  assumes trans_less: "cmp a b = Less \<Longrightarrow> cmp b c = Less \<Longrightarrow> cmp a c = Less"
-    and greater_iff_sym_less: "\<And>b a. cmp b a = Greater \<longleftrightarrow> cmp a b = Less"
+  fixes cmp :: \<open>'a \<Rightarrow> 'a \<Rightarrow> comp\<close>
+  assumes refl [simp]: \<open>\<And>a. cmp a a = Equiv\<close>
+    and trans_equiv: \<open>\<And>a b c. cmp a b = Equiv \<Longrightarrow> cmp b c = Equiv \<Longrightarrow> cmp a c = Equiv\<close>
+  assumes trans_less: \<open>cmp a b = Less \<Longrightarrow> cmp b c = Less \<Longrightarrow> cmp a c = Less\<close>
+    and greater_iff_sym_less: \<open>\<And>b a. cmp b a = Greater \<longleftrightarrow> cmp a b = Less\<close>
 begin
 
 text \<open>Dual properties\<close>
 
 lemma trans_greater:
-  "cmp a c = Greater" if "cmp a b = Greater" "cmp b c = Greater"
+  \<open>cmp a c = Greater\<close> if \<open>cmp a b = Greater\<close> \<open>cmp b c = Greater\<close>
   using that greater_iff_sym_less trans_less by blast
 
 lemma less_iff_sym_greater:
-  "cmp b a = Less \<longleftrightarrow> cmp a b = Greater"
+  \<open>cmp b a = Less \<longleftrightarrow> cmp a b = Greater\<close>
   by (simp add: greater_iff_sym_less)
 
 text \<open>The equivalence part\<close>
 
 lemma sym:
-  "cmp b a = Equiv \<longleftrightarrow> cmp a b = Equiv"
+  \<open>cmp b a = Equiv \<longleftrightarrow> cmp a b = Equiv\<close>
   by (metis (full_types) comp.exhaust greater_iff_sym_less)
 
 lemma reflp:
-  "reflp (\<lambda>a b. cmp a b = Equiv)"
+  \<open>reflp (\<lambda>a b. cmp a b = Equiv)\<close>
   by (rule reflpI) simp
 
 lemma symp:
-  "symp (\<lambda>a b. cmp a b = Equiv)"
+  \<open>symp (\<lambda>a b. cmp a b = Equiv)\<close>
   by (rule sympI) (simp add: sym)
 
 lemma transp:
-  "transp (\<lambda>a b. cmp a b = Equiv)"
+  \<open>transp (\<lambda>a b. cmp a b = Equiv)\<close>
   by (rule transpI) (fact trans_equiv)
 
 lemma equivp:
-  "equivp (\<lambda>a b. cmp a b = Equiv)"
+  \<open>equivp (\<lambda>a b. cmp a b = Equiv)\<close>
   using reflp symp transp by (rule equivpI)
 
 text \<open>The strict part\<close>
 
 lemma irreflp_less:
-  "irreflp (\<lambda>a b. cmp a b = Less)"
+  \<open>irreflp (\<lambda>a b. cmp a b = Less)\<close>
   by (rule irreflpI) simp
 
 lemma irreflp_greater:
-  "irreflp (\<lambda>a b. cmp a b = Greater)"
+  \<open>irreflp (\<lambda>a b. cmp a b = Greater)\<close>
   by (rule irreflpI) simp
 
 lemma asym_less:
-  "cmp b a \<noteq> Less" if "cmp a b = Less"
+  \<open>cmp b a \<noteq> Less\<close> if \<open>cmp a b = Less\<close>
   using that greater_iff_sym_less by force
 
 lemma asym_greater:
-  "cmp b a \<noteq> Greater" if "cmp a b = Greater"
+  \<open>cmp b a \<noteq> Greater\<close> if \<open>cmp a b = Greater\<close>
   using that greater_iff_sym_less by force
 
 lemma asymp_less:
-  "asymp (\<lambda>a b. cmp a b = Less)"
-  using irreflp_less by (auto intro: asympI dest: asym_less)
+  \<open>asymp (\<lambda>a b. cmp a b = Less)\<close>
+  using irreflp_less by (auto dest: asym_less)
 
 lemma asymp_greater:
-  "asymp (\<lambda>a b. cmp a b = Greater)"
-  using irreflp_greater by (auto intro!: asympI dest: asym_greater)
+  \<open>asymp (\<lambda>a b. cmp a b = Greater)\<close>
+  using irreflp_greater by (auto dest: asym_greater)
 
 lemma trans_equiv_less:
-  "cmp a c = Less" if "cmp a b = Equiv" and "cmp b c = Less"
+  \<open>cmp a c = Less\<close> if \<open>cmp a b = Equiv\<close> and \<open>cmp b c = Less\<close>
   using that
   by (metis (full_types) comp.exhaust greater_iff_sym_less trans_equiv trans_less)
 
 lemma trans_less_equiv:
-  "cmp a c = Less" if "cmp a b = Less" and "cmp b c = Equiv"
+  \<open>cmp a c = Less\<close> if \<open>cmp a b = Less\<close> and \<open>cmp b c = Equiv\<close>
   using that
   by (metis (full_types) comp.exhaust greater_iff_sym_less trans_equiv trans_less)
 
 lemma trans_equiv_greater:
-  "cmp a c = Greater" if "cmp a b = Equiv" and "cmp b c = Greater"
+  \<open>cmp a c = Greater\<close> if \<open>cmp a b = Equiv\<close> and \<open>cmp b c = Greater\<close>
   using that by (simp add: sym [of a b] greater_iff_sym_less trans_less_equiv)
 
 lemma trans_greater_equiv:
-  "cmp a c = Greater" if "cmp a b = Greater" and "cmp b c = Equiv"
+  \<open>cmp a c = Greater\<close> if \<open>cmp a b = Greater\<close> and \<open>cmp b c = Equiv\<close>
   using that by (simp add: sym [of b c] greater_iff_sym_less trans_equiv_less)
 
 lemma transp_less:
-  "transp (\<lambda>a b. cmp a b = Less)"
+  \<open>transp (\<lambda>a b. cmp a b = Less)\<close>
   by (rule transpI) (fact trans_less)
 
 lemma transp_greater:
-  "transp (\<lambda>a b. cmp a b = Greater)"
+  \<open>transp (\<lambda>a b. cmp a b = Greater)\<close>
   by (rule transpI) (fact trans_greater)
 
 text \<open>The reflexive part\<close>
 
 lemma reflp_not_less:
-  "reflp (\<lambda>a b. cmp a b \<noteq> Less)"
+  \<open>reflp (\<lambda>a b. cmp a b \<noteq> Less)\<close>
   by (rule reflpI) simp
 
 lemma reflp_not_greater:
-  "reflp (\<lambda>a b. cmp a b \<noteq> Greater)"
+  \<open>reflp (\<lambda>a b. cmp a b \<noteq> Greater)\<close>
   by (rule reflpI) simp
 
 lemma quasisym_not_less:
-  "cmp a b = Equiv" if "cmp a b \<noteq> Less" and "cmp b a \<noteq> Less"
+  \<open>cmp a b = Equiv\<close> if \<open>cmp a b \<noteq> Less\<close> and \<open>cmp b a \<noteq> Less\<close>
   using that comp.exhaust greater_iff_sym_less by auto
 
 lemma quasisym_not_greater:
-  "cmp a b = Equiv" if "cmp a b \<noteq> Greater" and "cmp b a \<noteq> Greater"
+  \<open>cmp a b = Equiv\<close> if \<open>cmp a b \<noteq> Greater\<close> and \<open>cmp b a \<noteq> Greater\<close>
   using that comp.exhaust greater_iff_sym_less by auto
 
 lemma trans_not_less:
-  "cmp a c \<noteq> Less" if "cmp a b \<noteq> Less" "cmp b c \<noteq> Less"
+  \<open>cmp a c \<noteq> Less\<close> if \<open>cmp a b \<noteq> Less\<close> \<open>cmp b c \<noteq> Less\<close>
   using that by (metis comp.exhaust greater_iff_sym_less trans_equiv trans_less)
 
 lemma trans_not_greater:
-  "cmp a c \<noteq> Greater" if "cmp a b \<noteq> Greater" "cmp b c \<noteq> Greater"
+  \<open>cmp a c \<noteq> Greater\<close> if \<open>cmp a b \<noteq> Greater\<close> \<open>cmp b c \<noteq> Greater\<close>
   using that greater_iff_sym_less trans_not_less by blast
 
 lemma transp_not_less:
-  "transp (\<lambda>a b. cmp a b \<noteq> Less)"
+  \<open>transp (\<lambda>a b. cmp a b \<noteq> Less)\<close>
   by (rule transpI) (fact trans_not_less)
 
 lemma transp_not_greater:
-  "transp (\<lambda>a b. cmp a b \<noteq> Greater)"
+  \<open>transp (\<lambda>a b. cmp a b \<noteq> Greater)\<close>
   by (rule transpI) (fact trans_not_greater)
 
 text \<open>Substitution under equivalences\<close>
 
 lemma equiv_subst_left:
-  "cmp z y = comp \<longleftrightarrow> cmp x y = comp" if "cmp z x = Equiv" for comp
+  \<open>cmp z y = comp \<longleftrightarrow> cmp x y = comp\<close> if \<open>cmp z x = Equiv\<close> for comp
 proof -
-  from that have "cmp x z = Equiv"
+  from that have \<open>cmp x z = Equiv\<close>
     by (simp add: sym)
   with that show ?thesis
     by (cases comp) (auto intro: trans_equiv trans_equiv_less trans_equiv_greater)
 qed
 
 lemma equiv_subst_right:
-  "cmp x z = comp \<longleftrightarrow> cmp x y = comp" if "cmp z y = Equiv" for comp
+  \<open>cmp x z = comp \<longleftrightarrow> cmp x y = comp\<close> if \<open>cmp z y = Equiv\<close> for comp
 proof -
-  from that have "cmp y z = Equiv"
+  from that have \<open>cmp y z = Equiv\<close>
     by (simp add: sym)
   with that show ?thesis
     by (cases comp) (auto intro: trans_equiv trans_less_equiv trans_greater_equiv)
@@ -160,10 +160,10 @@ qed
 
 end
 
-typedef 'a comparator = "{cmp :: 'a \<Rightarrow> 'a \<Rightarrow> comp. comparator cmp}"
+typedef 'a comparator = \<open>{cmp :: 'a \<Rightarrow> 'a \<Rightarrow> comp. comparator cmp}\<close>
   morphisms compare Abs_comparator
 proof -
-  have "comparator (\<lambda>_ _. Equiv)"
+  have \<open>comparator (\<lambda>_ _. Equiv)\<close>
     by standard simp_all
   then show ?thesis
     by auto
@@ -171,17 +171,17 @@ qed
 
 setup_lifting type_definition_comparator
 
-global_interpretation compare: comparator "compare cmp"
+global_interpretation compare: comparator \<open>compare cmp\<close>
   using compare [of cmp] by simp
 
-lift_definition flat :: "'a comparator"
-  is "\<lambda>_ _. Equiv" by standard simp_all
+lift_definition flat :: \<open>'a comparator\<close>
+  is \<open>\<lambda>_ _. Equiv\<close> by standard simp_all
 
 instantiation comparator :: (linorder) default
 begin
 
-lift_definition default_comparator :: "'a comparator"
-  is "\<lambda>x y. if x < y then Less else if x > y then Greater else Equiv"
+lift_definition default_comparator :: \<open>'a comparator\<close>
+  is \<open>\<lambda>x y. if x < y then Less else if x > y then Greater else Equiv\<close>
   by standard (auto split: if_splits)
 
 instance ..
@@ -193,8 +193,8 @@ text \<open>A rudimentary quickcheck setup\<close>
 instantiation comparator :: (enum) equal
 begin
 
-lift_definition equal_comparator :: "'a comparator \<Rightarrow> 'a comparator \<Rightarrow> bool"
-  is "\<lambda>f g. \<forall>x \<in> set Enum.enum. f x = g x" .
+lift_definition equal_comparator :: \<open>'a comparator \<Rightarrow> 'a comparator \<Rightarrow> bool\<close>
+  is \<open>\<lambda>f g. \<forall>x \<in> set Enum.enum. f x = g x\<close> .
 
 instance
   by (standard; transfer) (auto simp add: enum_UNIV)
@@ -202,23 +202,23 @@ instance
 end
 
 lemma [code]:
-  "HOL.equal cmp1 cmp2 \<longleftrightarrow> Enum.enum_all (\<lambda>x. compare cmp1 x = compare cmp2 x)"
+  \<open>HOL.equal cmp1 cmp2 \<longleftrightarrow> Enum.enum_all (\<lambda>x. compare cmp1 x = compare cmp2 x)\<close>
   by transfer (simp add: enum_UNIV)
 
 lemma [code nbe]:
-  "HOL.equal (cmp :: 'a::enum comparator) cmp \<longleftrightarrow> True"
+  \<open>HOL.equal (cmp :: 'a::enum comparator) cmp \<longleftrightarrow> True\<close>
   by (fact equal_refl)
 
 instantiation comparator :: ("{linorder, typerep}") full_exhaustive
 begin
 
 definition full_exhaustive_comparator ::
-  "('a comparator \<times> (unit \<Rightarrow> term) \<Rightarrow> (bool \<times> term list) option)
-    \<Rightarrow> natural \<Rightarrow> (bool \<times> term list) option"
-  where "full_exhaustive_comparator f s =
+  \<open>('a comparator \<times> (unit \<Rightarrow> term) \<Rightarrow> (bool \<times> term list) option)
+    \<Rightarrow> natural \<Rightarrow> (bool \<times> term list) option\<close>
+  where \<open>full_exhaustive_comparator f s =
     Quickcheck_Exhaustive.orelse
       (f (flat, (\<lambda>u. Code_Evaluation.Const (STR ''Comparator.flat'') TYPEREP('a comparator))))
-      (f (default, (\<lambda>u. Code_Evaluation.Const (STR ''HOL.default_class.default'') TYPEREP('a comparator))))"
+      (f (default, (\<lambda>u. Code_Evaluation.Const (STR ''HOL.default_class.default'') TYPEREP('a comparator))))\<close>
 
 instance ..
 
@@ -227,67 +227,67 @@ end
 
 subsection \<open>Fundamental comparator combinators\<close>
 
-lift_definition reversed :: "'a comparator \<Rightarrow> 'a comparator"
-  is "\<lambda>cmp a b. cmp b a"
+lift_definition reversed :: \<open>'a comparator \<Rightarrow> 'a comparator\<close>
+  is \<open>\<lambda>cmp a b. cmp b a\<close>
 proof -
-  fix cmp :: "'a \<Rightarrow> 'a \<Rightarrow> comp"
-  assume "comparator cmp"
+  fix cmp :: \<open>'a \<Rightarrow> 'a \<Rightarrow> comp\<close>
+  assume \<open>comparator cmp\<close>
   then interpret comparator cmp .
-  show "comparator (\<lambda>a b. cmp b a)"
+  show \<open>comparator (\<lambda>a b. cmp b a)\<close>
     by standard (auto intro: trans_equiv trans_less simp: greater_iff_sym_less)
 qed
 
-lift_definition key :: "('b \<Rightarrow> 'a) \<Rightarrow> 'a comparator \<Rightarrow> 'b comparator"
-  is "\<lambda>f cmp a b. cmp (f a) (f b)"
+lift_definition key :: \<open>('b \<Rightarrow> 'a) \<Rightarrow> 'a comparator \<Rightarrow> 'b comparator\<close>
+  is \<open>\<lambda>f cmp a b. cmp (f a) (f b)\<close>
 proof -
-  fix cmp :: "'a \<Rightarrow> 'a \<Rightarrow> comp" and f :: "'b \<Rightarrow> 'a"
-  assume "comparator cmp"
+  fix cmp :: \<open>'a \<Rightarrow> 'a \<Rightarrow> comp\<close> and f :: \<open>'b \<Rightarrow> 'a\<close>
+  assume \<open>comparator cmp\<close>
   then interpret comparator cmp .
-  show "comparator (\<lambda>a b. cmp (f a) (f b))"
+  show \<open>comparator (\<lambda>a b. cmp (f a) (f b))\<close>
     by standard (auto intro: trans_equiv trans_less simp: greater_iff_sym_less)
 qed
 
 
 subsection \<open>Direct implementations for linear orders on selected types\<close>
 
-definition comparator_bool :: "bool comparator"
-  where [simp, code_abbrev]: "comparator_bool = default"
+definition comparator_bool :: \<open>bool comparator\<close>
+  where [simp, code_abbrev]: \<open>comparator_bool = default\<close>
 
 lemma compare_comparator_bool [code abstract]:
-  "compare comparator_bool = (\<lambda>p q.
+  \<open>compare comparator_bool = (\<lambda>p q.
     if p then if q then Equiv else Greater
-    else if q then Less else Equiv)"
+    else if q then Less else Equiv)\<close>
   by (auto simp add: fun_eq_iff) (transfer; simp)+
 
-definition raw_comparator_nat :: "nat \<Rightarrow> nat \<Rightarrow> comp"
-  where [simp]: "raw_comparator_nat = compare default"
+definition raw_comparator_nat :: \<open>nat \<Rightarrow> nat \<Rightarrow> comp\<close>
+  where [simp]: \<open>raw_comparator_nat = compare default\<close>
 
 lemma default_comparator_nat [simp, code]:
-  "raw_comparator_nat (0::nat) 0 = Equiv"
-  "raw_comparator_nat (Suc m) 0 = Greater"
-  "raw_comparator_nat 0 (Suc n) = Less"
-  "raw_comparator_nat (Suc m) (Suc n) = raw_comparator_nat m n"
+  \<open>raw_comparator_nat (0::nat) 0 = Equiv\<close>
+  \<open>raw_comparator_nat (Suc m) 0 = Greater\<close>
+  \<open>raw_comparator_nat 0 (Suc n) = Less\<close>
+  \<open>raw_comparator_nat (Suc m) (Suc n) = raw_comparator_nat m n\<close>
   by (transfer; simp)+
 
-definition comparator_nat :: "nat comparator"
-  where [simp, code_abbrev]: "comparator_nat = default"
+definition comparator_nat :: \<open>nat comparator\<close>
+  where [simp, code_abbrev]: \<open>comparator_nat = default\<close>
 
 lemma compare_comparator_nat [code abstract]:
-  "compare comparator_nat = raw_comparator_nat"
+  \<open>compare comparator_nat = raw_comparator_nat\<close>
   by simp
 
-definition comparator_linordered_group :: "'a::linordered_ab_group_add comparator"
-  where [simp, code_abbrev]: "comparator_linordered_group = default"
+definition comparator_linordered_group :: \<open>'a::linordered_ab_group_add comparator\<close>
+  where [simp, code_abbrev]: \<open>comparator_linordered_group = default\<close>
 
 lemma comparator_linordered_group [code abstract]:
-  "compare comparator_linordered_group = (\<lambda>a b.
+  \<open>compare comparator_linordered_group = (\<lambda>a b.
     let c = a - b in if c < 0 then Less
-    else if c = 0 then Equiv else Greater)"
+    else if c = 0 then Equiv else Greater)\<close>
 proof (rule ext)+
   fix a b :: 'a
-  show "compare comparator_linordered_group a b =
+  show \<open>compare comparator_linordered_group a b =
     (let c = a - b in if c < 0 then Less
-       else if c = 0 then Equiv else Greater)"
+       else if c = 0 then Equiv else Greater)\<close>
     by (simp add: Let_def not_less) (transfer; auto)
 qed
 
